theories/Views/ViewSum.v
@@ -1,0 +1,49 @@
+Require Import MirrorCore.TypesI.
+Require Import MirrorCore.SymI.
+Require Import MirrorCore.Views.FuncView.
+Require Import MirrorCore.syms.SymSum.
+
+Section sum.
+  Context {typ : Type}.
+  Context {RT : @RType typ}.
+  Context {T U V : Type}.
+
+  Context {RSt : RSym T} {RSu : RSym U} {RSv : RSym V}.
+
+  Definition FuncView_left (FV_TU : FuncView U T)
+  : FuncView (U + V) T :=
+  {| f_insert := fun x => inl (f_insert x)
+   ; f_view := fun x => match x with
+                        | inl x => f_view x
+                        | _ => vNone
+                        end |}.
+
+  Theorem FuncViewOk_left (FV : FuncView U T) (FVo : FuncViewOk _ _ _)
+  : @FuncViewOk _ _ (@FuncView_left FV) _ _ (RSym_sum RSu RSv) _.
+  Proof.
+    constructor.
+    { simpl. destruct f; simpl.
+      { intros. rewrite fv_ok. split; congruence. }
+      { split; inversion 1. } }
+    { simpl. intros. rewrite fv_compat. reflexivity. }
+  Qed.
+
+  Definition FuncView_right (FV_TU : FuncView U T)
+  : FuncView (V + U) T :=
+  {| f_insert := fun x => inr (f_insert x)
+   ; f_view := fun x => match x with
+                        | inr x => f_view x
+                        | _ => vNone
+                        end |}.
+
+  Theorem FuncViewOk_right (FV : FuncView U T) (FVo : FuncViewOk _ _ _)
+  : @FuncViewOk _ _ (@FuncView_right FV) _ _ (RSym_sum RSv RSu) _.
+  Proof.
+    constructor.
+    { simpl. destruct f; simpl.
+      { split; inversion 1. }
+      { intros. rewrite fv_ok. split; congruence. } }
+    { simpl. intros. rewrite fv_compat. reflexivity. }
+  Qed.
+
+End sum.
